README.md
@@ -71,7 +71,7 @@ This repository contains the following case studies:
 * [hocap](theories/hocap): Formalizations of the concurrent bag and concurrent
   runners libraries from the [HOCAP paper](https://dl.acm.org/citation.cfm?id=2450283)
   (by Dan Frumin). See the associated [README](theories/hocap/README.md).
-* [array-based_queuing-lock](/theories/array_based_queuing_lock): Proof of
+* [array-based_queuing_lock](/theories/array_based_queuing_lock): Proof of
   safety of an implementation of the array-based queuing lock. This example is
   also covered in the chapter ["Case study: The Array-Based Queueing
   Lock"](https://iris-project.org/tutorial-pdfs/iris-lecture-notes.pdf#section.10)
